lib/zoo_persistent/parray_1.mli
@@ -1,9 +1,9 @@
 type 'a t
 
 val make :
-  int -> 'a -> 'a t
+  ('a -> 'a -> bool) -> int -> 'a -> 'a t
 
 val get :
   'a t -> int -> 'a
 val set :
-  'a t -> ('a -> 'a -> bool) -> int -> 'a -> 'a t
+  'a t -> int -> 'a -> 'a t
